newio/Free.Sig.fst
@@ -4,13 +4,25 @@ open FStar.List.Tot.Base
 
 open Free
 
-type cmds = | Openfile | Read | Close | GetTrace
-
 assume val file_descr : eqtype
+
+type cmds =
+  | Requires
+  | Openfile
+  | Read
+  | Close
+  | GetTrace
+
+let _req_cmds (x:cmds) : bool = x = Requires
+type req_cmds : Type0 = x:cmds{_req_cmds x} 
+unfold let req_args (x:req_cmds) : Type = pure_pre 
+unfold let req_res (x:req_cmds) (pre:req_args x) : Type = squash pre
+(** fails here because universe problems **)
+let req_sig : op_sig req_cmds = { args = req_args; res = req_res; }
 
 (** the io free monad does not contain the GetTrace step **)
 let _io_cmds x : bool = x = Openfile || x = Read || x = Close
-type io_cmds : Type = x:cmds{_io_cmds x}
+type io_cmds : Type0 = x:cmds{_io_cmds x}
 
 unfold let io_args (cmd:io_cmds) : Type =
   match cmd with
@@ -24,15 +36,20 @@ unfold let io_res (cmd:io_cmds) : Type =
   | Read -> string
   | Close -> unit
 
-let io_resm (cmd:io_cmds) = option (io_res cmd)
+let io_resm (cmd:io_cmds) (arg:io_args cmd) = option (io_res cmd)
 
 let io_sig : op_sig io_cmds = { args = io_args; res = io_resm; }
 
+
+type pio_cmds : Type = x:cmds{_io_cmds x || _req_cmds x}
+#set-options "--print_universes"
+let pio_sig : op_sig pio_cmds = add_sig cmds #_io_cmds #_req_cmds io_sig req_sig
+
 noeq
 type event =
-  | EOpenfile : a:io_args Openfile -> (r:io_resm Openfile) -> event
-  | ERead     : a:io_args Read     -> (r:io_resm Read)     -> event
-  | EClose    : a:io_args Close    -> (r:io_resm Close)    -> event
+  | EOpenfile : a:io_sig.args Openfile -> (r:io_sig.res Openfile a) -> event
+  | ERead     : a:io_sig.args Read     -> (r:io_sig.res Read a)     -> event
+  | EClose    : a:io_sig.args Close    -> (r:io_sig.res Close a)    -> event
 
 type trace = list event
 
@@ -50,23 +67,18 @@ to the trace from the heap. **)
 at extraction, they have to be careful to link it directly with the
 primitives, and not with the wrapped version, otherwise, they will
 suffer a performance penalty. **)
-let inst_res (x:inst_cmds) =
+let inst_arg (x:inst_cmds) = 
+  match x with
+  | GetTrace -> unit
+
+let inst_res (x:inst_cmds) (arg:inst_arg x) =
   match x with
   | GetTrace -> list event
 
-let inst_sig : op_sig inst_cmds = {
-  args = (fun (x:inst_cmds) -> match x with
-    | GetTrace -> unit) ;
-  res = inst_res
-}
+let inst_sig : op_sig inst_cmds = { args = inst_arg; res = inst_res }
 
-let iio_sig : op_sig cmds = add_sig cmds io_sig inst_sig
-
-let args (cmd:cmds) : Type = iio_sig.args cmd
-let res (cmd:cmds)  : (x:Type{x == iio_sig.res cmd}) =
-  admit ();
-  if cmd = GetTrace then inst_res cmd
-  else io_resm cmd
+type iio_cmds : Type = x:cmds{_io_cmds x || x = GetTrace}
+let iio_sig : op_sig iio_cmds = add_sig cmds io_sig inst_sig
 
 type io a = free io_cmds io_sig a
 let io_return (x:'a) : io 'a =
@@ -76,15 +88,15 @@ let io_bind (#a:Type) (#b:Type) l k : io b =
   free_bind io_cmds io_sig a b l k
 
 // THE IIO FREE MONAD
-type iio a = free cmds iio_sig a
+type iio a = free iio_cmds iio_sig a
 let iio_return (x:'a) : iio 'a =
-  free_return cmds iio_sig 'a x
+  free_return iio_cmds iio_sig 'a x
 
 let iio_bind (#a:Type) (#b:Type) l k : iio b =
-  free_bind cmds iio_sig a b l k
+  free_bind iio_cmds iio_sig a b l k
 
 // OTHER TYPES & UTILS
-type action_type = (cmd : io_cmds) & (args cmd)
+type action_type = (cmd : io_cmds) & (io_sig.args cmd)
 
 type monitorable_prop = (history:trace) -> (action:action_type) -> Tot bool
 
@@ -97,7 +109,7 @@ let convert_event_to_action (e:event) : action_type =
 let convert_call_to_event
   (cmd:io_cmds)
   (arg:io_args cmd)
-  (r:io_resm cmd) =
+  (r:io_resm cmd arg) =
   match cmd with
   | Openfile -> EOpenfile arg r
   | Read -> ERead arg r
@@ -125,7 +137,7 @@ unfold
 let apply_changes (history local_events:trace) : Tot trace =
   (List.rev local_events) @ history
 
-let destruct_event (e:event) : ( cmd:io_cmds & io_args cmd & io_resm cmd )  =
+let destruct_event (e:event) : ( cmd:io_cmds & (arg:io_args cmd) & io_resm cmd arg )  =
   match e with
   | EOpenfile arg res -> (| Openfile, arg, res |)
   | ERead arg res -> (| Read, arg, res |)
@@ -152,10 +164,10 @@ unfold let io_pre (cmd:io_cmds) (arg:io_args cmd) (h:trace) : Type0 =
 
 (** This file is replaced during linking with a file that contains the real
 implementation of the commands. **)
-let io_call (cmd:io_cmds) (arg:io_args cmd) : io (io_resm cmd) =
+let io_call (cmd:io_cmds) (arg:io_sig.args cmd) : io (iio_sig.res cmd arg) =
   Call cmd arg Return
 
 (** Since we can lift from io to iio, `iio_call` should be used only for 
 `GetTrace`. **)
-let iio_call (cmd:cmds) (arg:args cmd) : iio (res cmd) =
+let iio_call (cmd:iio_cmds) (arg:iio_sig.args cmd) : iio (iio_sig.res cmd arg) =
   Call cmd arg Return
