newio/DMFree.IO.fst
@@ -9,9 +9,8 @@ open Hist
 open DMFree
 include Free.Sig
 
-unfold let io_wps (cmd:io_cmds) (arg:io_args cmd) : hist #event (io_resm cmd) = fun p h ->
+unfold let io_wps (cmd:io_cmds) (arg:io_sig.args cmd) : hist #event (io_sig.res cmd arg) = fun p h ->
   match cmd with
- // | GetTrace -> p [] h
   | _ -> io_pre cmd arg h /\ (forall r. p [convert_call_to_event cmd arg r] r)
 
 let theta #a = theta #a #io_cmds #io_sig #event io_wps
@@ -21,7 +20,7 @@ let dm_return = dm_return io_cmds io_sig event io_wps
 let dm_bind = dm_bind io_cmds io_sig event io_wps
 let dm_subcomp = dm_subcomp io_cmds io_sig event io_wps
 let dm_if_then_else = dm_if_then_else io_cmds io_sig event io_wps
-let lift_pure_dm = lift_pure_dm io_cmds io_sig event io_wps
+//let lift_pure_dm = lift_pure_dm io_cmds io_sig event io_wps
 
 total
 reifiable
