newio/Free.fst
@@ -1,27 +1,18 @@
 module Free
 
 noeq
-type op_sig (op:Type u#a) = {
+type op_sig (op:Type0) = {
   args : op -> Type u#a;
-  res : op -> Type u#a;
+  res : (cmd:op) -> args cmd -> Type u#b;
 }
 
 noeq
-type free (op:Type0) (s:op_sig op) (a:Type) : Type =
-| Call : (l:op) -> s.args l -> cont:(s.res l -> free op s a) -> free op s a
-| PartialCall : (pre:pure_pre) -> cont:((squash pre) -> free op s a) -> free op s a
+type free (op:Type) (s:op_sig op) (a:Type) : Type =
+| Call : (l:op) -> arg:(s.args l) -> cont:(s.res l arg -> free op s a) -> free op s a
 | Return : a -> free op s a
 
 let free_return (op:Type) (s:op_sig op) (a:Type) (x:a) : free op s a =
   Return x
-
-let rec return_of (x:'a) (f:free 'op 's 'a) =
-  match f with
-  | Return x' -> x == x'
-  | Call cmd arg k ->
-     exists r'. return_of x (k r')
-  | PartialCall pre k ->
-     pre ==> return_of x (k ())
 
 let rec free_bind
   (op:Type)
@@ -36,9 +27,6 @@ let rec free_bind
   | Call cmd args fnc ->
       Call cmd args (fun i ->
         free_bind op s a b (fnc i) k)
-  | PartialCall pre fnc ->
-      PartialCall pre (fun _ ->
-        free_bind op s a b (fnc ()) k)
 
 let free_map
   (op:Type)
